added bottom time index to type system

Coq/ContextualCausality.v
@@ -12,50 +12,148 @@ Open Scope Z.
 
 (* Definition of the inference rules for contextual causality. *)
 
-Definition TimeEnv := list Z.
+Definition TimeB := option Z.
 
-Inductive CausalV : TimeEnv -> Z -> Var -> Prop :=
-| causal_V1 t t' g  : t <= t' -> CausalV (t :: g) t' V1
+Definition TimeEnv := list TimeB.
+
+Inductive tle : TimeB -> TimeB -> Prop:=
+| tle_bot t : tle None t
+| tle_notbot t1 t2 : t1 <= t2 -> tle (Some t1) (Some t2).
+
+Inductive tlt : TimeB -> TimeB -> Prop:=
+| tlt_bot t : tlt None (Some t)
+| tlt_notbot t1 t2 : t1 < t2 -> tlt (Some t1) (Some t2).
+
+
+Hint Constructors tle tlt.
+
+Definition tleb (t1 t2 : TimeB) : bool :=
+  match t1,t2 with
+    | Some t1', Some t2' => t1' <=? t2'
+    | None, _ => true
+    | _,_ => false
+  end.
+
+
+Lemma tleb_tle t1 t2 : tleb t1 t2 = true <-> tle t1 t2.
+Proof.
+  split; intro S; destruct t1, t2; simpl in *;inversion S;eauto using Zle_bool_imp_le, Zle_imp_le_bool. 
+Qed.
+
+Lemma tleb_tgt t1 t2 : tleb t1 t2 = false <-> tlt t2 t1.
+Proof.
+  admit.
+Qed.
+
+
+Inductive CausalV : TimeEnv -> TimeB -> Var -> Prop :=
+| causal_V1 t t' g  : tle t t' -> CausalV (t :: g) t' V1
 | causal_VS g v t t' : CausalV g t v -> CausalV (t' :: g) t (VS v).
 
+Definition tadd d : TimeB -> TimeB := liftM (fun t' => t' + d).
+Definition tsub d : TimeB -> TimeB := tadd (-d).
 
-Inductive CausalE : TimeEnv -> Z -> Exp -> Prop:= 
+
+Definition tadd' d : TimeB -> TimeB := tadd (Z.of_nat d).
+Definition tsub' d : TimeB -> TimeB := tsub (Z.of_nat d).
+
+Hint Unfold tsub tadd' tsub'.
+
+Inductive CausalE : TimeEnv -> TimeB -> Exp -> Prop:= 
  | causal_op t ts op args : all (CausalE ts t) args -> CausalE ts t (OpE op args)
- | causal_obs l t' t ts : t' <= t -> CausalE ts t (Obs l t')
+ | causal_obs l t' t ts : tle (Some t') t -> CausalE ts t (Obs l t')
  | causal_var t ts v : CausalV ts t v -> CausalE ts t (VarE v)
- | causal_acc t t' ts e1 e2 n : CausalE (map (fun x => x + Z.of_nat n) ts) (t + Z.of_nat n) e2
-                                -> CausalE (t' :: ts) t e1
+ | causal_acc t ts e1 e2 n : CausalE (map (tadd' n) ts) (tadd' n t) e2
+                                -> CausalE (None :: ts) t e1
                                 -> CausalE ts t (Acc e1 n e2)
   .
 
 
 
-Inductive CausalC : TimeEnv -> Z -> Contr -> Prop :=
+Inductive CausalC : TimeEnv -> TimeB -> Contr -> Prop :=
 | causal_zero ts t : CausalC ts t Zero
-| causal_translate ts t d c : CausalC (map (fun x => x - Z.of_nat d) ts) (t - Z.of_nat d) c
+| causal_translate ts t d c : CausalC (map (tsub' d) ts) (tsub' d t) c
                                      -> CausalC ts t (Translate d c)
 | causal_let ts t t' e c : CausalE ts t' e -> CausalC (t' :: ts) t c -> CausalC ts t (Let e c)
 | causal_scale ts t e c : CausalE ts t e -> CausalC ts t c -> CausalC ts t (Scale e c)
 | causal_both ts t c1 c2 : CausalC ts t c1 -> CausalC ts t c2 -> CausalC ts t (Both c1 c2)
-| causal_transfer t ts p1 p2 a : t <= 0 -> CausalC ts t (Transfer p1 p2 a)
-| causal_if ts t d e c1 c2 : CausalE ts 0 e -> CausalC ts t c1
-                             -> CausalC (map (fun x => x - Z.of_nat d) ts) (t - Z.of_nat d) c2
+| causal_transfer t ts p1 p2 a : tle t (Some 0) -> CausalC ts t (Transfer p1 p2 a)
+| causal_if ts t d e c1 c2 : CausalE ts (Some 0) e -> CausalC ts t c1
+                             -> CausalC (map (tsub' d) ts) (tsub' d t) c2
                              -> CausalC ts t (If e d c1 c2)
 .
 
 Hint Constructors CausalV CausalE CausalC.
 
-(* Contextual causality is 'open': i.e. it is (anti-)monotone w.r.t. ordering on time. *)
-
-Lemma CausalV_open t t' ts ts' (v : Var) : all2 Z.le ts' ts -> t <= t' -> CausalV ts t v -> CausalV ts' t' v.
+Lemma tle_refl t : tle t t.
 Proof.
-  intros Is I P. generalize dependent t. generalize dependent t'. generalize dependent ts. generalize dependent ts'.
-  induction v; intros; inversion P; subst.
-  - inversion Is. subst. constructor. omega.
-  - inversion Is. subst. constructor. eauto.
+  destruct t; auto using Z.le_refl.
 Qed.
 
-Lemma CausalE_open t t' ts ts' (e : Exp) : all2 Z.le ts' ts -> t <= t' -> CausalE ts t e -> CausalE ts' t' e.
+
+Lemma tle_trans n m p: tle n m -> tle m p -> tle n p.
+Proof.
+  intros A B. destruct n, m, p; inversion A; inversion B;
+  eauto using Z.le_trans. 
+Qed.
+
+Lemma tle_tadd n m d : tle n m -> tle (tadd d n) (tadd d m).
+Proof.
+  intro A. destruct n,m; inversion A; simpl; autounfold; constructor. omega.
+Qed.
+
+Lemma tle_tadd_rev n m d : tle (tadd d n) (tadd d m) -> tle n m.
+Proof.
+  intro A. destruct n,m; inversion A; simpl; autounfold; constructor. omega.
+Qed.
+
+
+Lemma tle_tadd' n m d : tle n m -> tle (tadd' d n) (tadd' d m).
+eauto using tle_tadd. Qed.
+
+
+Lemma tle_tsub' n m d : tle n m -> tle (tsub' d n) (tsub' d m).
+eauto 10 using tle_tadd. Qed.
+
+Lemma tle_tsub'_rev n m d : tle (tsub' d n) (tsub' d m) -> tle n m.
+eauto 10 using tle_tadd_rev. Qed.
+
+
+Lemma tadd_swap d e t : tadd d (tadd e t) = tadd e (tadd d t).
+Proof. 
+  destruct t; simpl;autounfold;f_equal. omega.
+Qed.
+
+Lemma tadd_tadd d e t : tadd d (tadd e t) = tadd (d + e) t.
+Proof. 
+  destruct t; simpl;autounfold;f_equal. omega.
+Qed.
+
+Lemma tadd_0 t : tadd 0 t = t.
+Proof. 
+  destruct t; simpl; autounfold;f_equal;omega.
+Qed.
+
+Lemma tadd'_0 t : tadd' 0 t = t.
+autounfold. simpl. apply tadd_0. Qed.
+
+Lemma tsub'_0 t : tsub' 0 t = t.
+autounfold. simpl. apply tadd_0. Qed.
+
+
+Hint Immediate tle_refl tadd_swap tadd_0 tadd'_0 tsub'_0.
+
+Hint Resolve tle_trans tle_tadd  tle_tadd' tle_tsub'.
+
+(* Contextual causality is 'open': i.e. it is (anti-)monotone w.r.t. ordering on time. *)
+
+Lemma CausalV_open t t' ts ts' (v : Var) : all2 tle ts' ts -> tle t t' -> CausalV ts t v -> CausalV ts' t' v.
+Proof.
+  intros Is I P. generalize dependent t. generalize dependent t'. generalize dependent ts. generalize dependent ts'.
+  induction v; intros; inversion P; subst; inversion Is; eauto.
+Qed.
+
+Lemma CausalE_open t t' ts ts' (e : Exp) : all2 tle ts' ts -> tle t t' -> CausalE ts t e -> CausalE ts' t' e.
 Proof.
   intros Is I P. generalize dependent t. generalize dependent t'.
   generalize dependent ts. generalize dependent ts'.
@@ -63,41 +161,41 @@ Proof.
   - induction args.
     * constructor.
     * inversion H3. inversion H. subst. constructor. eauto. apply IHargs. auto. constructor. auto. auto.
-  - omega.
+  - eauto.
   - eapply CausalV_open; eauto. 
-  - eapply IHe2; eauto. apply all2_map. intros. omega. assumption. omega.
-  - eapply IHe1 in H5.  apply H5; auto. constructor; auto. apply Z.le_refl. assumption.
+  - eapply IHe2;try eassumption;eauto using all2_map.
+  - eapply IHe1 in H5;eauto.
 Qed.
 
 
-Lemma CausalV_shift ts t v d : 0 <= d -> CausalV ts t v -> CausalV (map (fun x => x + d) ts) (t + d) v.
+Lemma CausalV_shift ts t v d : 0 <= d -> CausalV ts t v -> CausalV (map (tadd d) ts) (tadd d t) v.
 Proof.
-  intros D V. induction V;constructor. omega. assumption.
+  intros D V. induction V;constructor; auto.
 Qed.
 
-Lemma CausalE_shift ts t e d : 0 <= d -> CausalE ts t e -> CausalE (map (fun x => x + d) ts) (t + d) e.
+Lemma CausalE_shift ts t e d : 0 <= d -> CausalE ts t e -> CausalE (map (tadd d) ts) (tadd d t) e.
 Proof.
   intros D C. generalize dependent d. generalize dependent ts. generalize dependent t.
   induction e using Exp_ind';intros;inversion C; subst. 
   - constructor. do 2 eapply all_apply in H; eauto. 
     eapply all_mp in H3; try eapply H. do 2 eapply all_apply in H3; eauto.
-  - constructor. omega.
+  - constructor. destruct t; inversion H2; constructor. omega.
   - constructor. apply CausalV_shift;assumption.
   - econstructor.
     * eapply IHe2 in H3. rewrite map_map in *. 
-      rewrite <- Z.add_assoc. rewrite Z.add_comm with (n:=d0). rewrite Z.add_assoc. erewrite map_ext.
-      apply H3. intros. simpl. omega. omega.
+      unfold tadd' in *. rewrite tadd_swap. erewrite map_ext.
+      apply H3. simpl. auto. auto.
     * eapply IHe1 in H5. simpl in H5. apply H5. assumption.
 Qed.
 
-Corollary CausalE_shift_1 ts t e : CausalE ts t e -> CausalE (map (fun x => x + 1) ts) (t + 1) e.
+Corollary CausalE_shift_1 ts t e : CausalE ts t e -> CausalE (map (tadd 1) ts) (tadd 1 t) e.
 Proof.
   intros. apply CausalE_shift. omega. assumption.
 Qed.
 
-Definition env_until {A} t := all3 (B:=A) (fun t' x y => t' <= t -> x = y).
+Definition env_until {A} t := all3 (B:=A) (fun t' x y => tle t' t -> x = y).
 
-Lemma env_until_monotone {A} t ts f (e1 e2 : list A) : (forall x y, f x <= f y -> x <= y)
+Lemma env_until_monotone {A} t ts f (e1 e2 : list A) : (forall x y, tle (f x) (f y) -> tle x y)
                                                   -> env_until t ts e1 e2 -> env_until (f t) (map f ts) e1 e2.
 Proof.
   intros M U. induction U; constructor;auto. 
@@ -105,21 +203,33 @@ Qed.
 
 
 Lemma env_until_weaken {A} t t' ts (env1 env2 : list A) : 
-  env_until t ts env1 env2 -> t' <= t ->  env_until t' ts env1 env2.
+  env_until t ts env1 env2 -> tle t' t ->  env_until t' ts env1 env2.
 Proof.
-  intros U I. induction U;constructor;auto. intro. apply H. omega.
+  intros U I. induction U;constructor;auto. intro. apply H. eauto.
 Qed.
 
 Lemma env_until_weaken' {A} t ts ts' (env1 env2 : list A) : 
-  env_until t ts env1 env2 -> all2 Z.le ts ts' ->  env_until t ts' env1 env2.
+  env_until t ts env1 env2 -> all2 tle ts ts' ->  env_until t ts' env1 env2.
 Proof.
   intros U I. generalize dependent env1. generalize dependent env2. induction I;intros.
   inversion U. subst. constructor.
-  inversion U. subst. constructor. intros. apply H2. omega. 
+  inversion U. subst. constructor. intros. apply H2. eauto.
   unfold env_until in *. auto.
 Qed.
 
-Definition causalE ts t e := forall env1 env2 ext1 ext2, env_until t ts env1 env2 -> ext_until t ext1 ext2
+Definition ext_until' t (ext1 ext2 : ExtEnv) :=
+  match t with
+    | Some t' => ext_until t' ext1 ext2
+    | None => True
+  end.
+
+Lemma ext_until'_none e1 e2 : ext_until' None e1 e2.
+simpl. trivial.
+Qed.
+
+Hint Immediate ext_until'_none.
+
+Definition causalE ts t e := forall env1 env2 ext1 ext2, env_until t ts env1 env2 -> ext_until' t ext1 ext2
                                                         -> E[|e|] env1 ext1 = E[|e|]env2 ext2.
 
 (* Contextual causality implies semantic causality. *)
@@ -141,26 +251,30 @@ Proof.
   - eapply all_apply in H. apply all_mp with (Q:=causalE ts t) in H; auto. unfold causalE in *. 
     intros. simpl. do 6 eapply all_apply in H; eauto. erewrite map_rewrite; eauto. clear C.
     induction args; inversion H3; subst; constructor; auto.  apply IHargs; auto. inversion H. auto.
-  - unfold causalE. intros. simpl. unfold ext_until in *. rewrite H0; auto.
+  - unfold causalE. intros. simpl. inversion H2. subst. simpl in H0. unfold ext_until in *. rewrite H0; auto.
   - induction H2. 
     + unfold causalE. intros. inversion H0. subst. simpl. f_equal. auto.
     + unfold causalE in *. intros. inversion H. subst. simpl in *. eapply IHCausalV; eauto. 
-  - unfold causalE. intros. simpl. generalize dependent t'. 
+  - unfold causalE. intros. simpl.
     generalize dependent t. generalize dependent ts.
     generalize dependent ext1. generalize dependent ext2. unfold Fsem in *. induction d; intros.
-    + simpl. do 2 rewrite adv_ext_0. unfold causalE in IHe2. simpl in H3.
-      rewrite Z.add_0_r in H3. eapply IHe2; eauto. erewrite map_ext. rewrite map_id. assumption.
-      intros; omega.
+    + simpl. do 2 rewrite adv_ext_0. unfold causalE in IHe2. rewrite tadd'_0 in *.
+      eapply IHe2; eauto. erewrite map_ext. rewrite map_id. assumption.
+      auto. 
     + simpl. apply bind_equals. 
-      * do 2 rewrite adv_ext_step'. eapply IHd with (t := (t + 1)) (ts:= map (fun x => x + 1) ts); eauto. 
-        apply causal_acc with (t' := t' +1). 
-        rewrite succ_of_nat. rewrite map_map. rewrite map_ext with (g:=(fun x : Z => x + Z.of_nat (S d))).
-        assumption. intros. apply succ_of_nat. eapply CausalE_shift_1 in H5. simpl in H5. apply H5. 
-        rewrite map_map. rewrite succ_of_nat. erewrite map_ext. apply H3. intros. apply succ_of_nat.
-        apply env_until_monotone with (f := fun x => x + 1) in H. assumption. intros; omega.
-        rewrite Z.add_comm. rewrite <- ext_until_adv. 
-        do 2 rewrite adv_ext_iter. simpl. do 2 rewrite adv_ext_0. assumption.
+      * do 2 rewrite adv_ext_step'. eapply IHd with (t := tadd 1 t) (ts:= map (tadd 1) ts); eauto. 
+        apply causal_acc. 
+        rewrite map_map. erewrite map_ext. unfold tadd' in *. rewrite tadd_tadd. 
+        rewrite Nat2Z.inj_succ in *. unfold Z.succ in *.
+        eassumption. intros. autounfold. apply tadd_tadd.
+        eapply CausalE_shift_1 in H5. simpl in H5. apply H5. 
+        rewrite map_map. unfold tadd' in *. rewrite tadd_tadd. erewrite map_ext.
+        rewrite Nat2Z.inj_succ in *. unfold Z.succ in *.
+        apply H3. intros. apply tadd_tadd.
         eapply CausalE_shift_1 in H5. simpl in H5. apply H5.
+        apply env_until_monotone with (f := tadd 1) in H. assumption. intros. eauto using tle_tadd_rev.
+        destruct t;auto. simpl in *. rewrite Z.add_comm. rewrite <- ext_until_adv. 
+        do 2 rewrite adv_ext_iter. simpl. do 2 rewrite adv_ext_0. assumption.
       * intros. unfold causalE in IHe1. eapply IHe1. eassumption. constructor. auto. auto.
         do 2 rewrite adv_ext_iter. rewrite Pos2Z.add_neg_pos. rewrite Z.pos_sub_diag.
         do 2 rewrite adv_ext_0. assumption.
@@ -169,7 +283,7 @@ Qed.
 Lemma prec_of_nat t n : t - 1 - Z.of_nat n = t - Z.pos (Pos.of_succ_nat n).
 Proof. rewrite Zpos_P_of_succ_nat. omega. Qed.
 
-Lemma CausalC_empty ts t c tr i env ext : CausalC ts t c -> C[|c|]env ext = Some tr -> Z.of_nat i < t
+Lemma CausalC_empty ts t c tr i env ext : CausalC ts (Some t) c -> C[|c|]env ext = Some tr -> Z.of_nat i < t
                                            -> tr i = empty_trans.
 Proof.
   generalize dependent env. generalize dependent ext. generalize dependent tr. 
@@ -177,8 +291,9 @@ Proof.
   induction c;intros t ts i tr ext env C R I; simpl in *.
   - inversion R. reflexivity.
   - option_inv_auto. inversion C. subst. eapply IHc; eauto.
-  - inversion C. subst. eapply Z.lt_le_trans in H2;eauto. assert (0 = Z.of_nat 0) as Z by reflexivity.
-    rewrite Z in H2. rewrite <- Nat2Z.inj_lt in H2. inversion H2.
+  - inversion C. subst. inversion H2. subst. eapply Z.lt_le_trans in H1;eauto. 
+    assert (0 = Z.of_nat 0) as Z by reflexivity.
+    rewrite Z in H1. rewrite <- Nat2Z.inj_lt in H1. inversion H1.
   - option_inv_auto. inversion C. subst. rewrite <- scale_empty_trans with (r:=x). unfold scale_trace,compose.
     f_equal. eapply IHc; eauto.
   - option_inv_auto. inversion C. subst. unfold delay_trace. remember (leb n i) as L. destruct L;try reflexivity. 
@@ -197,19 +312,24 @@ Proof.
     induction n; intros.
     + simpl in *. destruct (E[|e|] env ext);tryfalse. destruct v;tryfalse. destruct b.
       * eapply IH1;eauto.
-      * eapply IHc2; eauto. rewrite Z.sub_0_r. assumption.
+      * eapply IHc2; eauto. rewrite Z.add_0_r. assumption.
     + simpl in *.  destruct (E[|e|] env ext);tryfalse. destruct v;tryfalse. destruct b.
       * eapply IH1 in R; eauto.
       * option_inv_auto. unfold delay_trace. remember (leb 1 i) as L. destruct L; try reflexivity.
         symmetry in HeqL. apply leb_complete in HeqL.
-        eapply IHn with (t:=(t - 1)) (ts:=map (fun x => x - 1) ts); auto. 
+        eapply IHn with (t:=(t - 1)) (ts:=map (tsub 1) ts); auto. 
         rewrite Nat2Z.inj_sub by assumption. 
-        simpl. omega. rewrite prec_of_nat. rewrite map_map. erewrite map_ext. eassumption. 
-        intros. simpl. apply prec_of_nat.
+        simpl. omega. autounfold. simpl. rewrite Z.add_opp_r. rewrite prec_of_nat. 
+        rewrite map_map. erewrite map_ext. eassumption. 
+        intros. autounfold. rewrite tadd_tadd. f_equal. rewrite Nat2Z.inj_succ. omega.
         intros. eapply IH1; eauto. omega. apply H0.
 Qed.
 
-
+Lemma CausalC_empty' ts t c tr i env ext : CausalC ts t c -> C[|c|]env ext = Some tr -> tlt (Some (Z.of_nat i)) t
+                                           -> tr i = empty_trans.
+Proof.
+  intros. destruct t; inversion H1. eapply CausalC_empty;eauto.
+Qed.
 
 Lemma all2_map_forall {A B} f l (P : A -> B -> Prop) : (forall x, P (f x) x) -> all2 P (map f l) l.
 Proof.
@@ -217,9 +337,9 @@ Proof.
 Qed.
 
 Lemma CausalC_sound' ts t t1 t2 i env1 env2 r1 r2 c : 
-  CausalC ts t c -> env_until (Z.of_nat i) ts env1 env2 ->
+  CausalC ts t c -> env_until (Some (Z.of_nat i)) ts env1 env2 ->
   ext_until (Z.of_nat i) r1 r2 -> C[|c|]env1 r1 = Some t1 -> C[|c|] env2 r2 = Some t2 ->
-  t <= Z.of_nat i -> t1 i = t2 i.
+  tle t (Some (Z.of_nat i)) -> t1 i = t2 i.
 Proof.
   intros C V X C1 C2 I. 
   generalize dependent ts. generalize dependent t. generalize dependent r1. generalize dependent r2.
@@ -230,20 +350,26 @@ Proof.
   - simpl in *. option_inv_auto. eapply IHc; eauto. constructor;auto.
     intro. rewrite CausalE_sound in H0;eauto. rewrite H0 in H2. 
     inversion H2. subst. reflexivity. eapply env_until_weaken; eassumption.
-    eapply ext_until_le. eassumption. omega.
+    destruct t';auto. simpl. inversion H. subst.
+    eapply ext_until_le. eassumption. assumption. 
   - simpl in *. inversion C1. inversion C2. reflexivity.
   - simpl in *. option_inv_auto. unfold scale_trace, compose. erewrite IHc; eauto.
     rewrite CausalE_sound in H5; eauto. rewrite H5 in H6. inversion H6. subst.
     destruct x3; tryfalse. rewrite H7 in H8. inversion H8. reflexivity.
-    eapply env_until_weaken. eassumption. omega.
-    eapply ext_until_le. eassumption. omega.
+    eapply env_until_weaken. eassumption. assumption.
+    destruct t;auto. inversion I. subst. eapply ext_until_le. eassumption. assumption.
   - simpl in *. option_inv_auto. unfold delay_trace. remember (leb n i) as L.
     destruct L; try reflexivity. symmetry in HeqL. apply leb_complete in HeqL.
-    eapply IHc; eauto. rewrite ext_until_adv. rewrite Nat2Z.inj_sub by assumption.
-    eapply ext_until_le. eassumption.  omega. rewrite Nat2Z.inj_sub by assumption. omega.
-    apply env_until_monotone with (f := (fun x1 : Z => x1 - Z.of_nat n)) in V. 
-    rewrite Nat2Z.inj_sub by assumption. apply V.
-    intros. omega.
+    eapply IHc with (t:= tsub' n t). eauto. rewrite ext_until_adv. rewrite Nat2Z.inj_sub by assumption.
+    eapply ext_until_le. eassumption.  omega. eauto. 
+    destruct t; inversion I;subst; simpl;autounfold; constructor. 
+    rewrite Nat2Z.inj_sub by assumption. omega.
+    apply env_until_monotone with (f := tsub' n) in V. 
+    eassumption.
+    intros. eauto using tle_tsub'_rev. 
+    rewrite Nat2Z.inj_sub by assumption. 
+    assert (tsub' n (Some (Z.of_nat i)) = Some (Z.of_nat i - Z.of_nat n)) as E by reflexivity.
+    rewrite <- E. eauto using env_until_monotone, tle_tsub'_rev.
   - simpl in *. option_inv_auto. unfold add_trace. f_equal; [eapply IHc1|eapply IHc2]; eauto.
   - simpl in *. apply CausalE_sound in H4. unfold causalE in *.
     assert (
@@ -253,43 +379,51 @@ Proof.
          forall r1 : ExtEnv,
          C[|c1|] env1 r1 = Some t1 ->
          ext_until (Z.of_nat i) r1 r2 ->
-         env_until (Z.of_nat i) ts env1 env2 -> t1 i = t2 i) as IH1.
-    intros. remember (t <=? Z.of_nat i0) as L. symmetry in HeqL. destruct L.
-    rewrite Z.leb_le in HeqL. eapply IHc1;eauto. rewrite Z.leb_gt in HeqL.
-    eapply CausalC_empty in H; eauto. eapply CausalC_empty in H0; eauto. 
-    rewrite H. rewrite H0. reflexivity.
-    
+         env_until (Some (Z.of_nat i)) ts env1 env2 -> t1 i = t2 i) as IH1.
+    intros. remember (tleb t (Some (Z.of_nat i0))) as L. symmetry in HeqL. destruct L.
+    rewrite tleb_tle in HeqL. eapply IHc1;eauto. rewrite tleb_tgt in HeqL.
+    eapply CausalC_empty' in H; eauto. eapply CausalC_empty' in H0; eauto. 
+    rewrite H. rewrite H0. reflexivity. 
+
     clear H6. clear IHc1.
     generalize dependent ts. generalize dependent t. generalize dependent r1. generalize dependent r2.
     generalize dependent env1. generalize dependent env2. generalize dependent i.
     generalize dependent t1. generalize dependent t2.
     induction n;intros.
     + simpl in *. rewrite H4 with (env2:=env2) (ext2:=r2) in C1;auto.
-      destruct (E[|e|] env2 r2);tryfalse. destruct v;tryfalse. rewrite Z.sub_0_r in *. 
+      destruct (E[|e|] env2 r2);tryfalse. destruct v;tryfalse. rewrite tsub'_0 in *. 
       destruct b; [eapply IH1|eapply IHc2]; eauto. erewrite map_ext. rewrite map_id. assumption.
-      intros. omega. 
-      eapply env_until_weaken. eassumption. omega.
+      intros. eauto.
+      eapply env_until_weaken. eassumption. constructor. omega.
       eapply ext_until_le. eassumption. omega.
     + simpl in *. rewrite H4 with (env2:=env2) (ext2:=r2) in C1;auto.
       destruct (E[|e|] env2 r2);tryfalse. destruct v;tryfalse. destruct b.
         eapply IH1; eauto.
         option_inv_auto. unfold delay_trace. remember (leb 1 i) as L. destruct L;try reflexivity.
         symmetry in HeqL. apply leb_complete in HeqL.
-        eapply IHn with (t:=t-1) (ts :=map (fun x => x - 1) ts);clear IHn;eauto. 
+        eapply IHn with (t:=tsub' 1 t) (ts :=map (tsub' 1) ts);clear IHn;eauto. 
         * rewrite ext_until_adv. eapply ext_until_le.
           apply X. rewrite Nat2Z.inj_sub by assumption. 
           assert (Z.of_nat 1 = 1) as E by reflexivity. rewrite E. omega. 
-        * rewrite Nat2Z.inj_sub by assumption. simpl. omega.
-        * apply env_until_monotone with (f:=fun x1 : Z => x1 - 1) in V. 
+        * rewrite Nat2Z.inj_sub by assumption. simpl. 
+          assert (Some (Z.of_nat i - 1) = tsub' 1 (Some (Z.of_nat i))) as E by reflexivity.
+          rewrite E. eapply tle_tsub'. assumption.
+        * apply env_until_monotone with (f:=tsub' 1) in V. 
           rewrite Nat2Z.inj_sub by assumption. apply V.
-          intros. omega. 
+          intros. eauto using tle_tsub'_rev.
         * intros. apply H4. 
-          eapply env_until_weaken'. eassumption. apply all2_map_forall. intro. omega.
+          eapply env_until_weaken'. eassumption. apply all2_map_forall. intro. 
+          destruct x1. simpl. autounfold. constructor. omega. auto.
           assumption.
-        * rewrite map_map. rewrite prec_of_nat. erewrite map_ext. apply H7. intros. apply prec_of_nat.
+        * assert (- Z.of_nat n + - Z.of_nat 1 = - Z.of_nat (S n)) as E
+            by (repeat rewrite Nat2Z.inj_succ; simpl; omega).
+          rewrite map_map. autounfold in *. 
+          rewrite tadd_tadd. erewrite map_ext. 
+          rewrite E. apply H7. intros. rewrite tadd_tadd. rewrite E. reflexivity.
         * intros. eapply IH1;eauto. 
-          eapply env_until_weaken'. eassumption. apply all2_map_forall. intro. omega.
-        * eapply env_until_weaken. eassumption. omega.
+          eapply env_until_weaken'. eassumption. apply all2_map_forall. intro. 
+          destruct x1. simpl. autounfold. constructor. omega. auto.
+        * eapply env_until_weaken. eassumption. constructor. omega.
         * eapply ext_until_le. eassumption. omega.
 Qed.
 
@@ -297,9 +431,9 @@ Qed.
 Theorem CausalC_sound t c : CausalC nil t c  -> causal c.
 Proof.
   intros C. unfold causal. intros. 
-  remember (t <=? Z.of_nat d) as L. symmetry in HeqL. destruct L.
-  - rewrite Z.leb_le in HeqL. eapply CausalC_sound'; eauto. constructor.
-  - rewrite Z.leb_gt in HeqL.
-    eapply CausalC_empty in H0; eauto. eapply CausalC_empty in H1; eauto. 
+  remember (tleb t (Some (Z.of_nat d))) as L. symmetry in HeqL. destruct L.
+  - rewrite tleb_tle in HeqL. eapply CausalC_sound'; eauto. constructor.
+  - rewrite tleb_tgt in HeqL.
+    eapply CausalC_empty' in H0; eauto. eapply CausalC_empty' in H1; eauto. 
     rewrite H0. rewrite H1. reflexivity.
 Qed.
