Coq/TimedTyping.v
@@ -11,20 +11,20 @@ Open Scope Z.
 
 (* Timed types *)
 
-Inductive TiTy := TimedType (ty : Ty) (ti : Z).
+Inductive TiTy := TimedType (ty : Ty) (ti : TimeB).
 
 Infix "^" := TimedType.
 
 (* Selector functions to extract the time and the type of a timed
 type. *)
 
-Definition time t := match t with TimedType _ ti => ti end.
-Definition type t := match t with TimedType ty _ => ty end.
+Definition time (t : TiTy)  := match t with TimedType _ ti => ti end.
+Definition type (t : TiTy) := match t with TimedType ty _ => ty end.
 
 (* Convenience function to add time to a timed type. *)
 
-Definition add_time d t := match t with TimedType ty ti => TimedType ty (ti + Z.of_nat d) end.
-Definition sub_time d t := match t with TimedType ty ti => TimedType ty (ti - Z.of_nat d) end.
+Definition add_time d (t : TiTy) := match t with TimedType ty ti => TimedType ty (tadd' d ti) end.
+Definition sub_time d (t : TiTy) := match t with TimedType ty ti => TimedType ty (tsub' d ti) end.
 
 (* A time timed time environment maps variables to timed types.  *)
 
@@ -35,34 +35,42 @@ Definition TiTyEnv := Env' TiTy.
 operators, expressions and contracts. *)
 
 Inductive TiTyV : TiTyEnv -> TiTy -> Var -> Prop :=
-| causal_V1 t t' g  : type t = type t' -> time t <= time t' -> TiTyV (t :: g) t' V1
+| causal_V1 t t' g  : type t = type t' -> tle (time t) (time t') -> TiTyV (t :: g) t' V1
 | causal_VS g v t t' : TiTyV g t v -> TiTyV (t' :: g) t (VS v).
 
 Definition TiTyOp (op : Op) (ts : list TiTy) (t:TiTy) : Prop
   := (all (fun t' => time t' = time t) ts) /\ TypeOp op (map type ts) (type t).
 
+Lemma TiTyOp_TypeOp op ts t ty tys : 
+  TypeOp op tys ty -> 
+  (all (fun t' => time t' = time t) ts) -> 
+  tys = map type ts -> ty = type t -> 
+  TiTyOp op ts t.
+Proof.
+  intros. subst. firstorder.
+Qed.
+
 Inductive TiTyE : TiTyEnv -> TiTy -> Exp -> Prop:= 
  | causal_op t ts ts' op args : TiTyOp op ts' t -> all2 (TiTyE ts) ts' args -> TiTyE ts t (OpE op args)
- | causal_obs l t' t ts : t' <= time t -> |-O l ∶ type t ->  TiTyE ts t (Obs l t')
+ | causal_obs l t' t ts : tle (Some t') (time t) -> |-O l ∶ type t ->  TiTyE ts t (Obs l t')
  | causal_var t ts v : TiTyV ts t v -> TiTyE ts t (VarE v)
- | causal_acc t t' ts e1 e2 n : type t = type t'
-                                -> TiTyE (map (add_time n) ts) (add_time n t) e2
-                                -> TiTyE (t' :: ts) t e1
-                                -> TiTyE ts t (Acc e1 n e2)
+ | causal_acc t ts e1 e2 n : TiTyE (map (add_time n) ts) (add_time n t) e2
+                             -> TiTyE (type t ^ None :: ts) t e1
+                             -> TiTyE ts t (Acc e1 n e2)
   .
 
 
 
-Inductive TiTyC : TiTyEnv -> Z -> Contr -> Prop :=
+Inductive TiTyC : TiTyEnv -> TimeB -> Contr -> Prop :=
 | causal_zero ts t : TiTyC ts t Zero
-| causal_translate ts t d c : TiTyC (map (sub_time d) ts) (t - Z.of_nat d) c
+| causal_translate ts t d c : TiTyC (map (sub_time d) ts) (tsub' d t) c
                                      -> TiTyC ts t (Translate d c)
 | causal_let ts t t' e c : TiTyE ts t' e -> TiTyC (t' :: ts) t c -> TiTyC ts t (Let e c)
 | causal_scale ts ti e c : TiTyE ts (REAL ^ ti) e -> TiTyC ts ti c -> TiTyC ts ti (Scale e c)
 | causal_both ts t c1 c2 : TiTyC ts t c1 -> TiTyC ts t c2 -> TiTyC ts t (Both c1 c2)
-| causal_transfer t ts p1 p2 a : t <= 0 -> TiTyC ts t (Transfer p1 p2 a)
-| causal_if ts t d e c1 c2 : TiTyE ts (BOOL ^ 0) e -> TiTyC ts t c1
-                             -> TiTyC (map (sub_time d) ts) (t - Z.of_nat d) c2
+| causal_transfer t ts p1 p2 a : tle t (Some 0) -> TiTyC ts t (Transfer p1 p2 a)
+| causal_if ts t d e c1 c2 : TiTyE ts (BOOL ^ Some 0) e -> TiTyC ts t c1
+                             -> TiTyC (map (sub_time d) ts) (tsub' d t) c2
                              -> TiTyC ts t (If e d c1 c2)
 .
 
@@ -98,8 +106,8 @@ Proof.
   - auto.
   - constructor. apply TiTyV_type. assumption.
   - constructor. 
-    + apply IHe1 in H6. simpl in *. rewrite H4 in *. assumption.
-    + apply IHe2 in H5. rewrite map_map in *. rewrite type_add_time in *. 
+    + apply IHe1 in H5. simpl in *. assumption.
+    + apply IHe2 in H3. rewrite map_map in *. rewrite type_add_time in *. 
       erewrite map_ext. eassumption. intros. simpl. rewrite type_add_time. reflexivity.
 Qed.
 
@@ -124,11 +132,11 @@ Proof.
   intro T. induction T;simpl in *; try rewrite H; auto.
 Qed.
 
-Lemma time_add_time d t :  time (add_time d t) = time t + Z.of_nat d.
+Lemma time_add_time d t :  time (add_time d t) = tadd' d (time t).
 Proof.
   destruct t. reflexivity.
 Qed.
-Lemma time_sub_time d t :  time (sub_time d t) = time t - Z.of_nat d.
+Lemma time_sub_time d t :  time (sub_time d t) = tsub' d (time t).
 Proof.
   destruct t. reflexivity.
 Qed.
@@ -146,9 +154,9 @@ Proof.
   - auto.
   - constructor. apply TiTyV_time. assumption.
   - econstructor. 
-    + apply IHe2 in H5. rewrite map_map in *. rewrite time_add_time in *. 
+    + apply IHe2 in H3. rewrite map_map in *. rewrite time_add_time in *. 
       erewrite map_ext. eassumption. intros. simpl. rewrite time_add_time. reflexivity.
-    + apply IHe1 in H6. simpl in *. eassumption.
+    + apply IHe1 in H5. simpl in *. eassumption.
 Qed.
 
 Hint Resolve TiTyE_type.
@@ -201,14 +209,14 @@ Proof.
   induction tys. reflexivity. simpl. f_equal. auto.
 Qed.
 
-Lemma map_add_time n tys tis : map (add_time n) tys ^^ tis = tys ^^ (map (fun t => t + Z.of_nat n) tis).
+Lemma map_add_time n tys tis : map (add_time n) tys ^^ tis = tys ^^ (map (tadd' n) tis).
 Proof.
   generalize dependent tis. induction tys;intros. reflexivity.
   destruct tis. reflexivity.
   simpl. rewrite IHtys. reflexivity.
 Qed.
 
-Lemma map_sub_time n tys tis : map (sub_time n) tys ^^ tis = tys ^^ (map (fun t => t - Z.of_nat n) tis).
+Lemma map_sub_time n tys tis : map (sub_time n) tys ^^ tis = tys ^^ (map (tsub' n) tis).
 Proof.
   generalize dependent tis. induction tys;intros. reflexivity.
   destruct tis. reflexivity.
@@ -227,19 +235,17 @@ Proof.
   - eauto.
   - econstructor. generalize dependent tis. generalize dependent ti. 
     induction H;intros;inversion H3; clear H3;subst;simpl; econstructor; eauto.
-  - apply causal_acc with (t' := t ^ t'). reflexivity. simpl. rewrite map_add_time. eauto.
-    specialize (IHTy1 ti (t' :: tis)). eauto.
+  - apply causal_acc. simpl. rewrite map_add_time. eauto.
+    specialize (IHTy1 ti (None :: tis)). eauto.
 Qed.
-
-Hint Resolve type_TiTyE.
 
 Theorem type_TiTyC tis tys ti  c : tys |-C c -> CausalC tis ti c -> TiTyC tys^^tis ti c.
 Proof.
   intros Ty Ti. generalize dependent tis. generalize dependent ti. 
-  induction Ty;intros;inversion Ti;subst;clear Ti;eauto.
-  - specialize (IHTy ti (t' :: tis)).  eauto.
+  induction Ty;intros;inversion Ti;subst;clear Ti;eauto using type_TiTyE.
+  - specialize (IHTy ti (t' :: tis)).  eauto using type_TiTyE.
   - econstructor. rewrite map_sub_time. eauto.
-  - econstructor; eauto. rewrite map_sub_time. eauto.
+  - econstructor; eauto using type_TiTyE. rewrite map_sub_time. eauto.
 Qed.
 
 
@@ -263,7 +269,7 @@ Proof.
   apply TiTyC_time in H. rewrite map_time in H; auto. destruct H. apply type_TiTyC;auto.
 Qed.
 
-Definition subtype (t1 t2 : TiTy) := type t1 = type t2 /\ time t1 <= time t2.
+Definition subtype (t1 t2 : TiTy) := type t1 = type t2 /\ tle (time t1) (time t2).
 
 Infix "<|" := subtype (at level 1).
 
@@ -273,7 +279,7 @@ Lemma subtype_type t1 t2 : t1 <| t2 -> type t1 = type t2.
 Proof.
   intros. unfold subtype in *. tauto.
 Qed.
-Lemma subtype_time t1 t2 : t1 <| t2 -> time t1 <= time t2.
+Lemma subtype_time t1 t2 : t1 <| t2 -> tle (time t1) (time t2).
 Proof.
   intros. unfold subtype in *. tauto.
 Qed.
@@ -285,7 +291,7 @@ Proof.
   intro H. induction H; simpl; f_equal; eauto.
 Qed.
 
-Lemma all_subtype_time ts1 ts2 : all2 subtype ts1 ts2 -> all2 Z.le (map time ts1) (map time ts2).
+Lemma all_subtype_time ts1 ts2 : all2 subtype ts1 ts2 -> all2 tle (map time ts1) (map time ts2).
 Proof.
   intro H. induction H; simpl; f_equal; eauto.
 Qed.
@@ -300,4 +306,148 @@ Proof.
 Qed.
 
 
+Definition inferObs (l : ObsLabel) : Ty :=
+  match l with
+    | LabR _ => REAL
+    | LabB _ => BOOL
+  end.
 
+
+Lemma inferObs_sound l : |-O l ∶ inferObs l.
+Proof.
+  destruct l; auto.
+Qed.
+
+Import ListNotations. 
+
+Definition tyeqb (t1 t2 : Ty) : bool :=
+  match t1, t2 with
+    | REAL, REAL => true
+    | BOOL, BOOL => true
+    | _,_ => false
+  end.
+
+Lemma tyeqb_iff t1 t2 : tyeqb t1 t2 = true <-> t1 = t2.
+Proof.
+  destruct t1;destruct t2; split;intro;simpl in *; congruence.
+Qed.
+
+Definition inferOp (op : Op) (args : list Ty) : option Ty :=
+  match op with
+    | Add => match args with [REAL;REAL] => Some REAL | _ => None end
+    | Sub => match args with [REAL;REAL] => Some REAL | _ => None end
+    | Mult => match args with [REAL;REAL] => Some REAL | _ => None end
+    | Div => match args with [REAL;REAL] => Some REAL | _ => None end
+    | And => match args with [BOOL;BOOL] => Some BOOL | _ => None end
+    | Or => match args with [BOOL;BOOL] => Some BOOL | _ => None end
+    | Less => match args with [REAL;REAL] => Some BOOL | _ => None end
+    | Leq => match args with [REAL;REAL] => Some BOOL | _ => None end
+    | Equal => match args with [REAL;REAL] => Some BOOL | _ => None end
+    | Not => match args with [BOOL] => Some BOOL | _ => None end
+    | Neg => match args with [REAL] => Some REAL | _ => None end
+    | BLit _ => match args with [] => Some BOOL | _ => None end
+    | RLit _ => match args with [] => Some REAL | _ => None end
+    | Cond => match args with [BOOL;t1;t2] => if tyeqb t1 t2 then Some t1 else None | _ => None end
+  end.
+
+Lemma inferOp_TypeOp op args ty : inferOp op args = Some ty <-> |-Op op ∶ args => ty.
+Proof.
+  destruct op; split; intro H; repeat (destruct args;try destruct t; simpl in *; try solve [inversion H;eauto]).
+Qed.
+
+Definition min_time (t1 t2 : option Z) : option Z :=
+  match t1,t2 with
+    | None, _ => t2
+    | _, None => t1
+    | Some t1', Some t2' => Some (Z.min t1' t2')
+  end.
+
+Definition min_times (ts : list (option Z)) : option Z :=fold_left min_time ts None.
+
+Definition add_timep d (t : TiTy) := match t with 
+                                        | TimedType ty (Some ti) => TimedType ty (Some (ti + Z.of_nat d))
+                                        | _ => t
+                                      end.
+
+Fixpoint inferE (env : TiTyEnv) (e:Exp) : option TiTy :=
+  match e with
+    | OpE op args => sequence (map (inferE env) args) >>=
+                              (fun args' => liftM (fun ty => ty ^ min_times (map time args')) 
+                                                  (inferOp op (map type args')))
+    | VarE v => lookupEnv v env
+    | Obs l i => Some (inferObs l ^ Some i)
+    | Acc f d z => inferE (map (add_timep d) env) z >>= 
+                  (fun t => inferE (type t ^ None :: env) f >>= 
+                  (fun t' => if tyeqb (type t) (type t') 
+                             then Some (type t ^ min_time (liftM (fun x => x + Z.of_nat d) (time t)) (time t')) 
+                             else None))
+  end.
+
+
+Definition instTiTy (t : TiTy) (t' : TiTy) : Prop := 
+  type t = type t' /\ (forall ti, time t = Some ti -> time t' = ti).
+
+Definition instTiTy_arb : TiTyP -> TiTy :=
+  (fun x => match x with 
+                  | ty ^ Some ti => ty ^ ti
+                  | ty ^ None => ty ^ 0
+                end).
+
+Lemma instTiTy_arb_sound t : instTiTy t (instTiTy_arb t).
+Proof.
+  destruct t. simpl. destruct ti; econstructor; eauto;firstorder; simpl in *; congruence.
+Qed.
+
+Hint Immediate inferObs_sound instTiTy_arb_sound.
+
+Lemma instTiTyEnv_arb_sound env : all2 instTiTy env (map instTiTy_arb env).
+Proof.
+  induction env;simpl;auto.
+Qed.
+
+
+Hint Immediate instTiTyEnv_arb_sound.
+
+Lemma lookupEnv_sound v env t t' :
+  instTiTy t t' -> lookupEnv v env = Some t -> 
+  exists env' : TiTyEnv, TiTyE env' t' (VarE v) /\ all2 instTiTy env env'.
+Proof.
+  generalize dependent v.
+  induction env;intros v T I;destruct v;tryfalse.
+  - simpl in I. inversion_clear I. eexists. split;[repeat constructor;reflexivity|auto].
+  - simpl in I. eapply IHenv in I; eauto. destruct I as [env' I]. destruct I as [I1 I2].
+    inversion_clear I1. eauto 6 using causal_var, causal_VS.
+Qed.
+
+Theorem inferE_sound env e t :
+   inferE env e = Some t -> 
+   forall t', instTiTy t t' -> 
+              exists env', TiTyE env' t' e /\ all2 instTiTy env env'.
+Proof.
+  intros I t' T. generalize dependent env. generalize dependent t. generalize dependent t'.
+  induction e using Exp_ind'; intros; simpl in *;option_inv_auto.
+  (* - repeat (eapply all_apply in H; eauto).  *)
+  (*   rewrite inferOp_TypeOp in *. eexists. split. econstructor. eapply TiTyOp_TypeOp.  *)
+  (*   eassumption. *)
+  (*   f_equal. *)
+
+  (*   split; [idtac|eapply H3]. *)
+  - admit.
+  - inversion I as [I']. clear I. subst. destruct T as [T1 T2]. simpl in *.
+    eexists. split; eauto. econstructor. erewrite T2; eauto. omega. rewrite <- T1. auto.
+  - eapply lookupEnv_sound;eauto.
+  - destruct x; destruct x0; simpl in H3. cases (tyeqb ty ty0) as E;tryfalse. apply tyeqb_iff in E.
+    inversion_clear H3. subst. eapply IHe1 in H2. eapply IHe2 in H0.
+    decompose [ex and] H2. decompose [ex and] H0. clear H0 H2.
+    eexists. split.
+    + econstructor. reflexivity
+Qed.
+
+Definition toTiTyP (t : TiTy) : TiTyP := TimedType (type t) (Some (time t)).
+
+
+Theorem inferE_complete env e t :
+  TiTyE env t e -> inferE (map toTiTyP env) e = Some (toTiTyP t).
+Proof.
+  admit.
+Qed.
